Examples/Exchanger.v
@@ -148,32 +148,6 @@ Definition Posts {A T} (i : Name T) : SRelt T A :=
   fun _ _ => Precs i.
 Notation Pend i m := (Some (MkCASPend i m)).
 
-Variant VisPossStep {T F} {VF : Spec T F} : Poss VF -> ThreadEvent T F -> Poss VF -> Prop :=
-| VPCommitCall i A (m : F A) (x y : Poss VF) :
-  VF.(Step) x.(PState) (i, CallEv m) y.(PState) ->
-  x.(PCalls) i = CallPoss m ->
-  y.(PCalls) i = CallDone m ->
-  x.(PRets) i = RetIdle ->
-  y.(PRets) i = RetIdle ->
-  VisPossStep x (i, CallEv m) y
-| VPCommitRet i A (m : F A) v (x y : Poss VF) :
-  VF.(Step) x.(PState) (i, RetEv m v) y.(PState) ->
-  x.(PCalls) i = CallDone m ->
-  y.(PCalls) i = CallDone m ->
-  x.(PRets) i = RetIdle ->
-  y.(PRets) i = RetPoss m v ->
-  VisPossStep x (i, RetEv m v) y.
-
-Inductive VisPossSteps {T F} {VF : Spec T F} : Poss VF -> Trace (ThreadEvent T F) -> Poss VF -> Prop :=
-| VRefl x :
-    VisPossSteps x [] x
-| VStep x y z i e p :
-    VisPossStep x (i, e) y ->
-    differ_pointwise (PCalls x) (PCalls y) i ->
-    differ_pointwise (PRets x) (PRets y) i ->
-    VisPossSteps y p z ->
-    VisPossSteps x ((i, e) :: p) z.
-
 Notation UnderStep s i e t := (PointStep UnderThreadStep s (i, Some e) t).
 
 Variant ExchTran {T A} : Name T -> InterState (F A) (VE T A) -> Poss (VF T A) -> InterState (F A) (VE T A) -> Poss (VF T A) -> Prop :=
@@ -285,30 +259,6 @@ destruct H. psimpl.
 econstructor.
 exists x. exact H1.
 easy.
-Qed.
-
-Lemma erase_vis {T F} {VF : Spec T F} :
-  forall (x y : Poss VF) p,
-  VisPossSteps x p y ->
-  PossSteps x y.
-intros. induction H. constructor.
-cut (PossStep i x y).
-{
-  intros. econstructor.
-  exact H3.
-  intros. now rewrite H0.
-  intros. now rewrite H1.
-  easy.
-}
-clear - H. ddestruct H.
-{
-  eapply PCommitCall.
-  exact H. all: easy.
-}
-{
-  eapply PCommitRet.
-  exact H. all: easy.
-}
 Qed.
 
 (* Tactics *)
@@ -831,69 +781,6 @@ Lemma float_lift {T A} {PT PF : SPrec T A}:
       (fun _ _ => LiftSPrec PF)) =
   (fun (b : bool) _ _ => LiftSPrec (if b then PT else PF)).
 extensionality b. now destruct b.
-Qed.
-
-Definition comInvPoss {T F} {VF : Spec T F} i (ρ : Poss VF) {A} (m : F A) (s : State VF) : Poss VF := {|
-  PState := s;
-  PCalls j := if i =? j then CallDone m else PCalls ρ j;
-  PRets j := PRets ρ j
-|}.
-
-Definition comRetPoss {T F} {VF : Spec T F} i (ρ : Poss VF) {A} (m : F A) (s : State VF) v : Poss VF := {|
-  PState := s;
-  PCalls := PCalls ρ;
-  PRets j := if i =? j then RetPoss m v else PRets ρ j
-|}.
-
-Lemma psteps_trans {T F} {VF : Spec T F} :
-  forall (x y z : Poss VF) p q,
-  VisPossSteps x p y ->
-  VisPossSteps y q z ->
-  VisPossSteps x (p ++ q) z.
-intros. induction H. easy.
-eapply VStep with (i:=i).
-4: now apply IHVisPossSteps.
-all: easy.
-Qed.
-
-Lemma retStep {T F} {VF : Spec T F} :
-  forall i (x z : Poss VF) p A (m : F A) v (y : State VF),
-  VisPossSteps x p z ->
-  (PCalls z i = CallDone m /\
-   PRets z i = RetIdle /\
-   VF.(Step) (PState z) (i, RetEv m v) y) ->
-  VisPossSteps x (p ++ [(i, RetEv m v)]) (comRetPoss i z m y v).
-intros.
-eapply psteps_trans.
-exact H.
-eapply VStep with
-  (i:=i). 4: constructor.
-psimpl.
-eapply VPCommitRet with
-  (m:=m) (v:=v).
-all: try easy.
-cbn. now rewrite eqb_id.
-apply differ_pointwise_trivial.
-Qed.
-
-Lemma callStep {T F} {VF : Spec T F} :
-  forall i (x z : Poss VF) p A (m : F A) (y : State VF),
-  VisPossSteps x p z ->
-  (PCalls z i = CallPoss m /\
-   PRets z i = RetIdle /\
-   VF.(Step) (PState z) (i, CallEv m) y) ->
-  VisPossSteps x (p ++ [(i, CallEv m)]) (comInvPoss i z m y).
-intros.
-eapply psteps_trans.
-exact H.
-eapply VStep with
-  (i:=i). 4: constructor.
-psimpl.
-eapply VPCommitCall with
-  (m:=m).
-all: try easy.
-cbn. now rewrite eqb_id.
-apply differ_pointwise_trivial.
 Qed.
 
 (* Rely lemmas *)
