Core/Scratch.v
@@ -1,3 +1,10 @@
-Definition K1 :=
-    forall (P : forall a, a = a -> Type),
-    P eq_refl
+Lemma foo :
+    forall P1 P2 Q1 Q2,
+    (P1 /\ Q1 \/ P2 /\ Q2) <->
+    ((P1 -> Q1) /\ (P2 -> Q2)).
+split; intros.
+{
+    split.
+    intros. destruct H.
+    easy. easy.
+}
