Core/VisPoss.v
@@ -1,0 +1,126 @@
+From Coq Require Import
+  Lists.List.
+Import ListNotations.
+
+From LHL.Core Require Import
+  LogicFacts
+  Traces
+  Specs
+  Logic.
+
+From LHL.Util Require Import
+  Util.
+
+Variant VisPossStep {T F} {VF : Spec T F} : Poss VF -> ThreadEvent T F -> Poss VF -> Prop :=
+| VPCommitCall i A (m : F A) (x y : Poss VF) :
+  VF.(Step) x.(PState) (i, CallEv m) y.(PState) ->
+  x.(PCalls) i = CallPoss m ->
+  y.(PCalls) i = CallDone m ->
+  x.(PRets) i = RetIdle ->
+  y.(PRets) i = RetIdle ->
+  VisPossStep x (i, CallEv m) y
+| VPCommitRet i A (m : F A) v (x y : Poss VF) :
+  VF.(Step) x.(PState) (i, RetEv m v) y.(PState) ->
+  x.(PCalls) i = CallDone m ->
+  y.(PCalls) i = CallDone m ->
+  x.(PRets) i = RetIdle ->
+  y.(PRets) i = RetPoss m v ->
+  VisPossStep x (i, RetEv m v) y.
+
+Inductive VisPossSteps {T F} {VF : Spec T F} : Poss VF -> Trace (ThreadEvent T F) -> Poss VF -> Prop :=
+| VRefl x :
+    VisPossSteps x [] x
+| VStep x y z i e p :
+    VisPossStep x (i, e) y ->
+    differ_pointwise (PCalls x) (PCalls y) i ->
+    differ_pointwise (PRets x) (PRets y) i ->
+    VisPossSteps y p z ->
+    VisPossSteps x ((i, e) :: p) z.
+
+Lemma erase_vis {T F} {VF : Spec T F} :
+  forall (x y : Poss VF) p,
+  VisPossSteps x p y ->
+  PossSteps x y.
+intros. induction H. constructor.
+cut (PossStep i x y).
+{
+  intros. econstructor.
+  exact H3.
+  intros. now rewrite H0.
+  intros. now rewrite H1.
+  easy.
+}
+clear - H. ddestruct H.
+{
+  eapply PCommitCall.
+  exact H. all: easy.
+}
+{
+  eapply PCommitRet.
+  exact H. all: easy.
+}
+Qed.
+
+Definition comInvPoss {T F} {VF : Spec T F} i (ρ : Poss VF) {A} (m : F A) (s : State VF) : Poss VF := {|
+  PState := s;
+  PCalls j := if i =? j then CallDone m else PCalls ρ j;
+  PRets j := PRets ρ j
+|}.
+
+Definition comRetPoss {T F} {VF : Spec T F} i (ρ : Poss VF) {A} (m : F A) (s : State VF) v : Poss VF := {|
+  PState := s;
+  PCalls := PCalls ρ;
+  PRets j := if i =? j then RetPoss m v else PRets ρ j
+|}.
+
+
+Lemma psteps_trans {T F} {VF : Spec T F} :
+  forall (x y z : Poss VF) p q,
+  VisPossSteps x p y ->
+  VisPossSteps y q z ->
+  VisPossSteps x (p ++ q) z.
+intros. induction H. easy.
+eapply VStep with (i:=i).
+4: now apply IHVisPossSteps.
+all: easy.
+Qed.
+
+Lemma retStep {T F} {VF : Spec T F} :
+  forall i (x z : Poss VF) p A (m : F A) v (y : State VF),
+  VisPossSteps x p z ->
+  (PCalls z i = CallDone m /\
+   PRets z i = RetIdle /\
+   VF.(Step) (PState z) (i, RetEv m v) y) ->
+  VisPossSteps x (p ++ [(i, RetEv m v)]) (comRetPoss i z m y v).
+intros.
+eapply psteps_trans.
+exact H.
+eapply VStep with
+  (i:=i). 4: constructor.
+psimpl.
+eapply VPCommitRet with
+  (m:=m) (v:=v).
+all: try easy.
+cbn. now rewrite eqb_id.
+apply differ_pointwise_trivial.
+Qed.
+
+Lemma callStep {T F} {VF : Spec T F} :
+  forall i (x z : Poss VF) p A (m : F A) (y : State VF),
+  VisPossSteps x p z ->
+  (PCalls z i = CallPoss m /\
+   PRets z i = RetIdle /\
+   VF.(Step) (PState z) (i, CallEv m) y) ->
+  VisPossSteps x (p ++ [(i, CallEv m)]) (comInvPoss i z m y).
+intros.
+eapply psteps_trans.
+exact H.
+eapply VStep with
+  (i:=i). 4: constructor.
+psimpl.
+eapply VPCommitCall with
+  (m:=m).
+all: try easy.
+cbn. now rewrite eqb_id.
+apply differ_pointwise_trivial.
+Qed.
