Examples/AtomicStackSpec.v
@@ -1,0 +1,52 @@
+From LHL.Core Require Import
+  Program
+  Specs
+  Logic.
+
+From LHL.Util Require Import
+  Tactics
+  TransUtil
+  Util.
+
+Variant AtomicStackSig {A} : ESig :=
+| Push (v : A) : AtomicStackSig unit
+| Pop : AtomicStackSig (option A).
+Arguments AtomicStackSig : clear implicits.
+
+Record AtomicStackPend {T A} := MkStkPend {
+  StkRetTy : Type;
+  StkName : Name T;
+  StkCall : AtomicStackSig A StkRetTy
+}.
+Arguments AtomicStackPend : clear implicits.
+Arguments MkStkPend {T A StkRetTy}.
+
+Variant AtomicStackState {T A} :=
+| AtomicStackDef (vs : list A) (m : option (AtomicStackPend T A)).
+Arguments AtomicStackState : clear implicits.
+
+Variant AtomicStackStep {T A} : AtomicStackState T A -> ThreadEvent T (AtomicStackSig A) -> AtomicStackState T A -> Prop :=
+| AtomicStackCall i R (m : _ R) vs : AtomicStackStep
+  (AtomicStackDef vs None)
+  (i, CallEv m)
+  (AtomicStackDef vs (Some (MkStkPend i m)))
+| RetPush i v vs : AtomicStackStep
+    (AtomicStackDef vs (Some (MkStkPend i (Push v))))
+    (i, RetEv (Push v) tt)
+    (AtomicStackDef (v :: vs) None)
+| RetPopPass i v vs : AtomicStackStep
+    (AtomicStackDef (v :: vs) (Some (MkStkPend i Pop)))
+    (i, RetEv Pop (Some v))
+    (AtomicStackDef vs None)
+| RetPopFail i : AtomicStackStep
+    (AtomicStackDef nil (Some (MkStkPend i Pop)))
+    (i, RetEv Pop None)
+    (AtomicStackDef nil None).
+
+Program Definition atomicStackSpec {T A} : Spec T (AtomicStackSig A) := {|
+  State := AtomicStackState T A;
+  Step := AtomicStackStep;
+  Init := AtomicStackDef nil None
+|}.
+
+Admit Obligations.
