Examples/EBStack.v
@@ -1,0 +1,1149 @@
+From LHL.Core Require Import
+  ProgramRules
+  Program
+  LogicFacts
+  SingConds
+  Program
+  ProgramRules
+  ProgramFacts
+  Traces
+  Tensor
+  Logic
+  Specs
+  VisPoss.
+
+From LHL.Util Require Import
+  TransUtil
+  Tactics
+  Util.
+
+From LHL.Examples Require Import
+  ExchangerSpec
+  AtomicStackSpec
+  WaitFreeStackSpec.
+
+From Coq Require Import
+  Lists.List
+  Logic.FunctionalExtensionality
+  Logic.PropExtensionality.
+Import ListNotations.
+
+Unset Printing Records.
+
+Definition E A :=
+  ExchSig (option A) |+| WaitFreeStackSig A.
+
+Definition VE T A : Spec T (E A) :=
+  tensorSpec exchSpec wfStackSpec.
+
+Definition F A := AtomicStackSig A.
+
+Definition VF T A : Spec T (F A) :=
+  atomicStackSpec.
+
+Definition push {A} (v : A) : Prog (E A) unit :=
+  loop (
+    b <- call (WFPush v);
+    match b with
+    | PASS tt => ret (Break tt)
+    | FAIL =>
+        b <- call (Exch (Some v));
+        match b with
+        | Some None => ret (Break tt)
+        | _ => ret Continue
+        end
+    end
+  ).
+
+(* TODO: fix FAIL case *)
+Definition pop {A} : Prog (E A) (option A) :=
+  loop (
+    b <- call WFPop;
+    match b with
+    | PASS v => ret (Break v)
+    | FAIL =>
+        b <- call (Exch None);
+        match b with
+        | Some (Some v) => ret (Break (Some v))
+        | _ => ret Continue
+        end
+    end
+  ).
+
+Definition EBStack A : Impl (E A) (F A) :=
+  fun _ m => match m with
+  | Push v => push v
+  | Pop => pop
+  end.
+
+Definition Prec T A := SPrec (VE T A) (VF T A).
+Definition Relt T A := SRelt (VE T A) (VF T A).
+Definition Post T A R := R -> SRelt (VE T A) (VF T A).
+
+Notation stkSt s := (RState (snd s)).
+Notation exchSt s := (LState (snd s)).
+
+Notation IStep s i e t :=
+  (InterStep (EBStack _) s (i, UEvent (Some e)) t).
+
+Variant EBTran {T A} : Relt T A :=
+| StkCallPush s x t i v :
+    IStep s i (CallEv (inr (WFPush v))) t ->
+    EBTran s x t x
+| StkPushPass s x t y i v :
+    IStep s i (RetEv (inr (WFPush v)) (PASS tt)) t ->
+    VisPossSteps x [(i, CallEv (Push v)); (i, RetEv (Push v) tt)] y ->
+    EBTran s x t y
+| StkPushFail s x t i v :
+    IStep s i (RetEv (inr (WFPush v)) FAIL) t ->
+    EBTran s x t x
+| StkOffer s x t i v :
+    IStep s i (CallEv (inl (Exch v))) t ->
+    EBTran s x t x
+| StkRevoke s x t i v :
+    IStep s i (RetEv (inl (Exch v)) None) t ->
+    EBTran s x t x
+| StkPushAccept s x t y i j v :
+    IStep s i (RetEv (inl (Exch (Some v))) (Some None)) t ->
+    VisPossSteps
+      x
+      [(i, CallEv (Push v)); (i, RetEv (Push v) tt);
+       (j, CallEv Pop); (j, RetEv Pop (Some v))]
+      y ->
+    EBTran s x t y
+| StkPopAccept s x t y i j v :
+    IStep s i (RetEv (inl (Exch None)) (Some (Some v))) t ->
+    VisPossSteps
+      x
+      [(i, CallEv (Push v)); (i, RetEv (Push v) tt);
+       (j, CallEv Pop); (j, RetEv Pop (Some v))]
+      y ->
+    EBTran s x t y
+| StkPushFinish s x t i v :
+    IStep s i (RetEv (inl (Exch (Some v))) (Some None)) t ->
+    EBTran s x t x
+| StkPushConflict s x t i v w :
+    IStep s i (RetEv (inl (Exch (Some v))) (Some (Some w))) t ->
+    EBTran s x t x
+| StkPopFinish s x t i v :
+    IStep s i (RetEv (inl (Exch None)) (Some (Some v))) t ->
+    EBTran s x t x
+| StkNoOp s x t i :
+    InterStep (EBStack _) s (i, UEvent None) t ->
+    EBTran s x t x.
+
+Definition Guar {T A} : Relt T A :=
+  EBTran.
+
+Definition Rely {T A} : Relt T A :=
+  SRTC EBTran.
+
+Record Waiting {T A R} (i : Name T) (m : F A R)
+  (x : Poss (VF T A))
+:= {
+  call_waiting : PCalls x i = CallPoss m;
+  ret_waiting : PRets x i = RetIdle;
+}.
+
+Record Done {T A R} (i : Name T) (m : F A R) (v : R)
+  (x : Poss (VF T A))
+:= {
+  call_done : PCalls x i = CallDone m;
+  ret_done : PRets x i = RetPoss m v
+}.
+
+Record Offered1 {T A} (i : Name T) (v : option A)
+  (s : InterState (F A) (VE T A)) (x : Poss (VF T A))
+:= {
+  exch_offered : exchSt s = ExchDef {i => v} {};
+}.
+
+Record Offered2 {T A} (i j : Name T) (v w : option A)
+  (s : InterState (F A) (VE T A)) (x : Poss (VF T A))
+:= {
+  exchs_offered : exchSt s = ExchDef {i => v, j => w} {};
+}.
+
+Record Accepted {T A} (i j : Name T) (v : A)
+  (s : InterState (F A) (VE T A)) (x : Poss (VF T A))
+:= {
+  accepted : exchSt s = ExchDef {j => None} {i => Some v};
+  push_done : Done i (Push v) tt x;
+  (* pop_done : Done i Pop (Some v) x *)
+}.
+
+Record Conflicted {T A} (i j : Name T) (v w : A)
+  (s : InterState (F A) (VE T A)) (x : Poss (VF T A))
+:= {
+  conflicted : exchSt s = ExchDef {i => Some v} {j => Some w}
+}.
+
+Record Inv {T A}
+  (s : InterState (F A) (VE T A)) (x : Poss (VF T A))
+:= {
+  state_consistent :
+    exists vs pu,
+      stkSt s = WaitFreeStackDef vs pu /\
+      PState x = AtomicStackDef vs None;
+  pop_offer_waiting :
+    forall i os cs,
+      exchSt s = ExchDef os cs ->
+      (i, None) ∈ os ->
+      Waiting i Pop x
+}.
+
+Lemma foldProg {E A} :
+  forall p : Prog E A,
+  match p with
+  | Return v => Return v
+  | Bind m k => Bind m k
+  | NoOp p => NoOp p
+  end = p.
+intros.
+destruct p; easy.
+Qed.
+
+Lemma stepLoopBind {E E' A B} e `{SigCoercion E' E} :
+  forall m : E' A,
+  forall C : A -> Prog E (ControlFlow B),
+  loopAux e (x <- call m; C x) = (x <- call m; loopAux e (C x)). 
+intros.
+rewrite frobProgId with (p:=loopAux _ _). cbn.
+rewrite frobProgId with (p:= x <- call m; _). cbn.
+f_equal. extensionality x.
+Admitted.
+
+Lemma stepLoopBreak {E A} e :
+  forall v : A,
+  loopAux e (ret (E:=E) (Break v)) = ret v.
+intros. now rewrite frobProgId at 1.
+Qed.
+
+Lemma stepLoopCont {E A} e :
+  loopAux e (ret (E:=E) (Continue (A:=A))) = NoOp (loop e).
+intros. now rewrite frobProgId at 1.
+Qed.
+
+Lemma stepCall {E E' A B} {m : E' A} {k : A -> Prog E B} `{SigCoercion E' E} :
+  (x <- call m; k x) = Bind (coerceOp _ m) k.
+rewrite frobProgId at 1. cbn.
+f_equal. extensionality x.
+rewrite frobProgId at 1. simpl.
+apply foldProg.
+Qed.
+
+Lemma eq_inj {A} {x y : A} :
+  eq x = eq y -> x = y.
+intros. now rewrite H.
+Qed.
+
+Ltac eq_inj H :=
+  apply eq_inj in H; subst.
+
+Ltac begin_commit :=
+  unfold Commit, LiftSPrec; intros.
+
+Ltac inst_eqs :=
+  repeat match goal with
+  | [ H : forall (x : Poss (VF _ _)), eq ?y = eq x -> _ |- _ ] =>
+      specialize (H ?y eq_refl); psimpl
+  end.
+
+Ltac begin_stable :=
+  unfold Stable, stablePost, stableRelt, sub, subRelt;
+  unfold ReltToPrec, LiftSPrec, LiftSRelt;
+  intros; psimpl.
+
+Ltac simp_sets :=
+  repeat match goal with
+  | [ H : {?i => ?v} = {} |- _ ] =>
+      now apply disj_cons in H
+  | [ H : {} = {?i => ?v} |- _ ] =>
+      symmetry in H;
+      now apply disj_cons in H
+  | [ H : insert ?x ?xs = insert ?y ?ys |- _ ] =>
+      let H2 := fresh in
+      let H3 := fresh in
+      apply insert_cong in H;
+      destruct H as [H2 H3];
+      ddestruct H2
+  | [ H : emp = emp |- _ ] =>
+      clear H
+  end.
+
+(* Lemma Waiting_tran {T A} :
+  forall (i : Name T) R (m : F A R),
+  forall s x t y,
+  Waiting i m x ->
+  Rely s x t y ->
+  (Waiting i m y \/
+   exists).
+Admitted. *)
+
+Lemma Done_stable {T A} :
+  forall (i : Name T) R (m : F A R),
+  forall s x t y v,
+  Done i m v x ->
+  Rely s x t y ->
+  Done i m v y.
+Admitted.
+
+Lemma push_correct {T A} {i : Name T} {v : A} :
+  VerifyProg i (LiftSRelt Rely) (LiftSRelt Guar)
+    (prComp (LiftSPrec Inv) (TInvoke (EBStack A) i _ (Push v)) ->> LiftSRelt Rely)
+    (push v)
+    (fun _ _ _ => LiftSPrec (fun s x =>
+      Inv s x /\
+      Returned i (Push v) tt s (eq x))).
+eapply weakenPrec with
+  (P:=fun _ _ => LiftSPrec (fun s x =>
+    Inv s x /\
+    Waiting i (Push v) x)).
+2:{
+  admit.
+}
+cut (
+  forall P,
+  P ==> (fun _ _ => LiftSPrec (fun s x =>
+    Inv s x /\
+    Waiting i (Push v) x)) ->
+    VerifyProg i (LiftSRelt Rely) (LiftSRelt Guar)
+      P
+      (push v)
+      (fun _ _ _ => LiftSPrec (fun s x =>
+        Inv s x /\
+        Returned i (Push v) tt s (eq x)))
+).
+{ intros. now apply H. }
+cofix rec. intros P impH. unfold push, loop.
+rewrite stepLoopBind, stepCall.
+eapply SafeBind with
+  (QI:=fun _ _ => LiftSPrec (fun s x =>
+    Inv s x /\
+    Waiting i (Push v) x))
+  (QR:=fun r _ _ => LiftSPrec (fun s x =>
+    Inv s x /\
+    match r with
+    | PASS tt => Done i (Push v) tt x
+    | FAIL => Waiting i (Push v) x
+    end)).
+{
+  clear rec impH. begin_stable.
+  specialize (H0 x1 eq_refl). psimpl.
+  exists x0. split. easy.
+  split.
+  {
+    admit.
+  }
+  {
+    admit.
+  }
+}
+{
+  clear rec impH. begin_stable.
+  specialize (H0 x1 eq_refl). psimpl.
+  exists x0. split. easy.
+  split.
+  {
+    admit.
+  }
+  {
+    destruct v0.
+    {
+      destruct v0.
+      eapply Done_stable.
+      exact H2. exact H0.
+    }
+    {
+      admit.
+    }
+  }
+}
+{
+  clear rec. begin_commit.
+  psimpl. apply impH in H.
+  clear impH. psimpl.
+  unfold LiftSPrec in H. psimpl.
+  exists (eq x).
+  split.
+  { now exists x. }
+  split.
+  {
+    intros. subst. exists σ.
+    repeat (constructor || easy).
+  }
+  split.
+  {
+    exists x. split. easy.
+    split.
+    {
+      destruct H7. psimpl.
+      ddestruct H2.
+      {
+        constructor.
+        {
+          eexists vs, _.
+          split. symmetry. exact x.
+          rewrite <- x3 in H. ddestruct H.
+          exact H7.
+        }
+        { now setoid_rewrite <- H6 at 1. }
+      }
+      {
+        constructor.
+        {
+          eexists vs, _.
+          split. symmetry. exact x.
+          rewrite <- x3 in H. ddestruct H.
+          exact H7.
+        }
+        { now setoid_rewrite <- H6 at 1. }
+      }
+    }
+    { easy. }
+  }
+  {
+    exists x. split. easy.
+    eq_inj H. apply StkCallPush with
+      (i:=i) (v:=v).
+    constructor.
+    {
+      constructor; cbn.
+      easy. intros. now rewrite H0.
+    }
+    { easy. }
+  }
+}
+clear impH.
+intros. destruct v0.
+{
+  clear rec.
+  destruct v0.
+  split.
+  {
+    begin_commit. do 5 destruct H.
+    clear H. psimpl. psimpl.
+    ddestruct H.
+    {
+      admit.
+    }
+    exists (eq (
+      comRetPoss i
+        (comInvPoss i
+          x3
+          (Push v)
+          (AtomicStackDef vs (Some (MkStkPend i (Push v)))))
+        (Push v)
+        (AtomicStackDef (v :: vs) None)
+        tt
+    )).
+    assert (
+      VisPossSteps
+        x3
+        ([(i, CallEv (Push v))] ++ [(i, RetEv (Push v) tt)])
+        (comRetPoss i
+          (comInvPoss i
+            x3
+            (Push v)
+            (AtomicStackDef vs (Some (MkStkPend i (Push v)))))
+          (Push v)
+          (AtomicStackDef (v :: vs) None)
+          tt)
+    ).
+    {
+      apply retStep.
+      apply callStep with (p:=[]).
+      constructor.
+      {
+        destruct H3, H4. psimpl.
+        rewrite <- x1 in H. ddestruct H.
+        rewrite H3. repeat (constructor || easy).
+      }
+      {
+        cbn. rewrite eqb_id.
+        destruct H4, H3. psimpl.
+        repeat (constructor || easy).
+      }
+    }
+    split.
+    { repeat eexists. }
+    split.
+    {
+      intros. subst.
+      eexists. split. easy.
+      eapply erase_vis. exact H.
+    }
+    split.
+    {
+      eexists. split. easy.
+      split.
+      {
+        destruct H3. psimpl.
+        constructor.
+        {
+          exists (v :: vs), None.
+          cbn. repeat (constructor || easy).
+        }
+        {
+          setoid_rewrite <- H7.
+          intros. apply pop_offer_waiting0
+            with (i:=i0) in H9. 2: easy.
+          assert (i <> i0).
+          {
+            unfold not. intros. subst.
+            destruct H4, H9.
+            rewrite call_waiting0 in call_waiting1.
+            ddestruct call_waiting1.
+          }
+          destruct H9.
+          constructor; cbn;
+          now rewrite eqb_nid.
+        }
+      }
+      {
+        constructor; cbn;
+        now rewrite eqb_id.
+      }
+    }
+    {
+      eexists. split. easy.
+      apply StkPushPass with
+        (i:=i) (v:=v).
+      {
+        constructor.
+        {
+          constructor; cbn.
+          easy. intros. now rewrite H0.
+        }
+        {
+          cbn. split. 2: easy.
+          rewrite <- x1, <- x at 1.
+          constructor.
+        }
+      }
+      { now eq_inj H8. }
+    }
+  }
+  {
+    rewrite stepLoopBreak. apply SafeReturn.
+    unfold sub, subRelt. intros. psimpl.
+    unfold LiftSPrec in H1. psimpl.
+    exists x3. destruct H3.
+    repeat (easy || constructor).
+    all: (subst; easy).
+  }
+}
+{
+  split.
+  {
+    clear rec. begin_commit.
+    do 5 destruct H. clear H.
+    psimpl. psimpl. exists (eq x3).
+    split.
+    { now exists x3. }
+    split.
+    {
+      intros. subst. eexists.
+      repeat (constructor || easy).
+    }
+    split.
+    {
+      exists x3. split. easy.
+      split.
+      {
+        destruct H3. psimpl.
+        constructor. ddestruct H.
+        {
+          eexists vs, _. split.
+          symmetry. exact x.
+          rewrite <- x4 in H3.
+          ddestruct H3. exact H8.
+        }
+        { now setoid_rewrite <- H7 at 1. }
+      }
+      { easy. }
+    }
+    {
+      eexists. split. easy.
+      eq_inj H8. apply StkPushFail with
+        (i:=i) (v:=v).
+      constructor.
+      {
+        constructor; cbn.
+        easy. intros. now rewrite H0.
+      }
+      { easy. }
+    }
+  }
+  {
+    rewrite stepLoopBind, stepCall.
+    eapply SafeBind with
+      (QI:=fun _ _ => LiftSPrec (fun s x =>
+        Inv s x /\
+        ((Waiting i (Push v) x /\
+          (Offered1 i (Some v) s x \/
+           exists j w, i <> j /\ Offered2 i j (Some v) w s x)) \/
+         (Done i (Push v) tt x /\
+          exists j, i <> j /\ Accepted i j v s x))))
+      (QR:=fun r _ _ => LiftSPrec (fun s x =>
+        Inv s x /\
+        (match r with
+         | Some None => Done i (Push v) tt x
+         | _ => Waiting i (Push v) x
+         end))).
+    {
+      clear rec. begin_stable.
+      specialize (H0 x1 eq_refl). psimpl.
+      exists x0. split. easy.
+      admit.
+    }
+    {
+      clear rec.
+      admit.
+    }
+    {
+      clear rec. begin_commit.
+      rewrite <- reltCompAssoc in H.
+      do 5 destruct H. clear H. do 2 psimpl.
+      ddestruct H. 2: destruct x1.
+      {
+        exists (eq x3).
+        split.
+        { repeat econstructor. }
+        split.
+        {
+          intros. subst.
+          repeat econstructor.
+        }
+        split.
+        {
+          exists x3. split. easy.
+          split.
+          {
+            destruct H3. psimpl.
+            constructor.
+            {
+              exists x2, x4.
+              rewrite <- H7 at 1. easy.
+            }
+            {
+              intros.
+              rewrite <- x in H8 at 1.
+              ddestruct H8. apply contains_invert in H9.
+              destruct H9. easy. now apply contains_contr in H8.
+            }
+          }
+          {
+            left. split. easy.
+            left. easy.
+          }
+        }
+        {
+          exists x3. split. easy.
+          eq_inj H. eapply StkOffer.
+          constructor; cbn.
+          {
+            constructor; cbn.
+            exact H1. intros. now rewrite H0.
+          }
+          {
+            rewrite <- x1, <- x at 1.
+            repeat (easy || constructor).
+          }
+        }
+      }
+      {
+        exists (eq x3).
+        split.
+        { repeat econstructor. }
+        split.
+        {
+          intros. subst.
+          repeat econstructor.
+        }
+        split.
+        {
+          exists x3. split. easy.
+          split.
+          {
+            destruct H3. psimpl.
+            constructor.
+            {
+              exists x1, x4.
+              rewrite <- H7 at 1. easy.
+            }
+            {
+              intros.
+              rewrite <- x in H9 at 1. ddestruct H9.
+              apply contains_invert in H10.
+              destruct H10. easy.
+              apply contains_invert in H9.
+              destruct H9. easy.
+              now apply contains_contr in H9.
+            }
+          }
+          {
+            left. split. easy.
+            right. exists i0, (Some a).
+            easy.
+          }
+        }
+        {
+          exists x3. split. easy.
+          eq_inj H8. eapply StkOffer.
+          constructor; cbn.
+          {
+            constructor; cbn.
+            exact H1. intros. now rewrite H0.
+          }
+          {
+            rewrite <- x2, <- x at 1.
+            repeat (easy || constructor).
+          }
+        }
+      }
+      {
+        exists (eq x3).
+        split.
+        { repeat econstructor. }
+        split.
+        {
+          intros. subst.
+          repeat econstructor.
+        }
+        split.
+        {
+          exists x3. split. easy.
+          split.
+          {
+            destruct H3. psimpl.
+            constructor.
+            {
+              exists x1, x4.
+              rewrite <- H7 at 1. easy.
+            }
+            {
+              intros.
+              symmetry in x2.
+              dec_eq_nats i1 i0.
+              {
+                apply pop_offer_waiting0 with (i:=i0) in x2.
+                2: apply contains_triv. easy.
+              }
+              {
+                rewrite <- x in H9 at 1. ddestruct H9.
+                apply contains_invert in H10.
+                destruct H10. ddestruct H9.
+                apply contains_invert in H9.
+                destruct H9. now ddestruct H9.
+                now apply contains_contr in H9.
+              }
+            }
+          }
+          {
+            left. split. easy.
+            right. exists i0, None.
+            easy.
+          }
+        }
+        {
+          exists x3. split. easy.
+          eq_inj H8. eapply StkOffer.
+          constructor; cbn.
+          {
+            constructor; cbn.
+            exact H1. intros. now rewrite H0.
+          }
+          {
+            rewrite <- x2, <- x at 1.
+            repeat (easy || constructor).
+          }
+        }
+      }
+    }
+    intros.
+    assert (v0 = Some None \/ v0 <> Some None).
+    {
+      destruct v0. destruct o.
+      now right. now left. now right.
+    }
+    destruct H. subst.
+    {
+      clear rec.
+      split.
+      {
+        begin_commit. do 5 destruct H.
+        clear H. do 2 psimpl.
+        destruct H3. psimpl. rename x into vs.
+        repeat match goal with
+        | [ H : ?P \/ ?Q |- _ ] =>
+            destruct H
+        | [ H : ?P /\ ?Q |- _ ] =>
+            destruct H
+        end; psimpl.
+        {
+          (*
+          revoke case is impossible here because
+          we have assumed the return value is
+          Some None. the revoke case is handled
+          in the v0 <> Some None branch
+          *)
+          destruct H9.
+          rewrite exch_offered0 in H at 1.
+          ddestruct H; simp_sets.
+        }
+        {
+          (* accept *)
+          destruct H10.
+          rewrite exchs_offered0 in H at 1.
+          remember (Some None). move Heqo at bottom.
+          ddestruct H; simp_sets. ddestruct Heqo.
+          rename x5 into j.
+          set (x3' :=
+            comRetPoss j
+              (comInvPoss j
+                (comRetPoss i
+                  (comInvPoss i
+                    x3
+                    (Push v)
+                    (AtomicStackDef vs (Some (MkStkPend i (Push v)))))
+                  (Push v)
+                  (AtomicStackDef (v :: vs) None)
+                  tt)
+                Pop
+                (AtomicStackDef (v :: vs) (Some (MkStkPend j Pop))))
+              Pop
+              (AtomicStackDef vs None)
+              (Some v)
+          ).
+          assert (
+            VisPossSteps
+              x3
+              ([] ++
+               [(i, CallEv (Push v))] ++ [(i, RetEv (Push v) tt)] ++
+               [(j, CallEv Pop)]      ++ [(j, RetEv Pop (Some v))])
+              x3'
+          ).
+          {
+            apply pop_offer_waiting0
+              with (i:=j)
+              in exchs_offered0.
+            2:{ rewrite insert_perm. apply contains_triv. }
+            destruct exchs_offered0.
+            repeat rewrite app_assoc.
+            apply retStep. apply callStep.
+            apply retStep. apply callStep.
+            constructor.
+            {
+              destruct H4. rewrite H8.
+              repeat (easy || constructor).
+            }
+            {
+              cbn. rewrite eqb_id. destruct H4.
+              repeat (easy || constructor).
+            }
+            {
+              cbn. rewrite eqb_nid; try easy.
+              repeat (easy || constructor).
+            }
+            {
+              cbn. rewrite eqb_id, eqb_nid.
+              repeat (easy || constructor).
+              easy.
+            } 
+          }
+          exists (eq x3').
+          split.
+          { repeat econstructor. }
+          split.
+          {
+            intros. subst.
+            exists x3. split. easy.
+            eapply erase_vis.
+            exact H10.
+          }
+          split.
+          {
+            exists x3'. split. easy.
+            split.
+            {
+              constructor.
+              {
+                exists vs, x1.
+                now rewrite <- H7 at 1.
+              }
+              {
+                intros. rewrite <- x in H11 at 1.
+                ddestruct H11. apply contains_invert in H12.
+                destruct H12. ddestruct H11.
+                now apply contains_contr in H11.
+              }
+            }
+            {
+              subst x3'.
+              constructor; cbn;
+              now rewrite eqb_id, eqb_nid.
+            }
+          }
+          {
+            exists x3'. split. easy.
+            eq_inj H11. eapply StkPushAccept
+              with (i:=i) (v:=v).
+            {
+              constructor; cbn.
+              {
+                constructor; cbn.
+                easy. intros. now rewrite H0.
+              }
+              {
+                rewrite exchs_offered0, <- x at 1.
+                repeat (easy || constructor).
+              }
+            }
+            { exact H10. }
+          }
+        }
+        {
+          (* finish *)
+          destruct H10.
+          exists (eq x3).
+          split.
+          { repeat econstructor. }
+          split.
+          {
+            intros. subst. eexists.
+            repeat constructor.
+          }
+          split.
+          {
+            exists x3. split. easy.
+            split.
+            {
+              constructor.
+              {
+                exists vs, x1.
+                now rewrite <- H7 at 1.
+              }
+              {
+                intros.
+                rewrite accepted0 in H at 1.
+                ddestruct H; simp_sets.
+                rewrite <- x in H10 at 1.
+                ddestruct H10.
+                now apply contains_contr in H11.
+              }
+            }
+            { easy. }
+          }
+          {
+            exists x3. split. easy.
+            eq_inj H10. eapply StkPushFinish
+              with (i:=i) (v:=v).
+            constructor.
+            {
+              constructor; cbn.
+              easy. intros. now rewrite H0.
+            }
+            { easy. }
+          }
+        }
+      }
+      {
+        rewrite stepLoopBreak.
+        apply SafeReturn.
+        unfold sub, subRelt.
+        intros. unfold LiftSPrec in H.
+        psimpl. exists x4. destruct H3.
+        repeat (easy || constructor).
+        all: (subst; easy).
+      }
+    }
+    {
+      split.
+      {
+        begin_commit.
+        repeat rewrite <- reltCompAssoc in H0.
+        do 5 destruct H0. clear H0. psimpl.
+        destruct H4. psimpl. rename x into vs.
+        destruct H5; destruct H5; psimpl.
+        {
+          remember v0.
+          move Heqo at bottom.
+          ddestruct H0; simp_sets.
+          {
+            assert (exists z, y = Some z).
+            {
+              clear - H. destruct y.
+              repeat econstructor.
+              easy.
+            }
+            psimpl. rename x4 into w.
+            exists (eq x3).
+            split.
+            { repeat econstructor. }
+            split.
+            {
+              intros. subst.
+              repeat econstructor.
+            }
+            split.
+            {
+              exists x3. split. easy.
+              split.
+              {
+                constructor.
+                {
+                  exists vs, x1.
+                  now rewrite <- H7 at 1.
+                }
+                {
+                  intros.
+                  rewrite <- x in H11 at 1.
+                  ddestruct H11.
+                  apply contains_invert in H12.
+                  destruct H12. ddestruct H11.
+                  now apply contains_contr in H11.
+                }
+              }
+              { easy. }
+            }
+            {
+              exists x3. split. easy.
+              eq_inj H11. eapply StkPushConflict
+                with (i:=i) (v:=v) (w:=w).
+              constructor; cbn.
+              {
+                constructor; cbn. easy.
+                intros. now rewrite H1.
+              }
+              {
+                rewrite <- x, <- x2 at 1.
+                repeat (easy || constructor).
+              }
+            }
+          }
+          {
+            assert (exists z, x2 = Some z).
+            {
+              clear - H. destruct x2.
+              repeat econstructor.
+              easy.
+            }
+            psimpl.
+            rename i0 into j.
+            rename x5 into w.
+            exists (eq x3).
+            split.
+            { repeat econstructor. }
+            split.
+            {
+              intros. subst.
+              repeat econstructor.
+            }
+            split.
+            {
+              exists x3. split. easy.
+              split.
+              {
+                constructor.
+                {
+                  exists vs, x1.
+                  now rewrite <- H7 at 1.
+                }
+                {
+                  intros.
+                  rewrite <- x in H11 at 1. ddestruct H11.
+                  now apply contains_contr in H12.
+                }
+              }
+              { easy. }
+            }
+            {
+              exists x3. split. easy.
+              eq_inj H11. eapply StkRevoke
+                with (i:=i) (v:= Some v).
+              constructor.
+              {
+                constructor; cbn.
+              }
+            }
+          }
+          {
+            admit.
+          }
+        }
+        {
+          admit.
+        }
+      }
+      {
+        eassert (
+          match v0 with
+          | Some None => ret (Break tt)
+          | _ => ret Continue
+          end = ret Continue
+        ).
+        {
+          destruct v0.
+          destruct o.
+          all: easy.
+        }
+        rewrite H0. clear H0.
+        rewrite stepLoopCont.
+        apply SafeNoOp with
+          (QS:=fun _ _ => LiftSPrec (fun s x =>
+            Inv s x /\
+            Waiting i (Push v) x)).
+        {
+          (* Inv and Waiting stable *)
+          admit.
+        }
+        {
+          unfold SilentStep. intros.
+          unfold LiftSPrec in H0.
+          repeat rewrite <- reltCompAssoc in H0.
+          do 5 destruct H0. clear H0. psimpl.
+          split.
+          {
+            exists x3. split. easy.
+            ddestruct H2. destruct H3. psimpl.
+            split.
+            {
+              constructor.
+              {
+                exists x4, x5.
+                easy.
+              }
+              {
+                admit.
+              }
+              {
+                admit.
+              }
+              {
+                admit.
+              }
+            }
+            {
+              destruct v0. destruct o.
+              all: easy.
+            }
+          }
+          {
+            exists x3. split. easy.
+            eq_inj H0. eapply StkNoOp.
+            split. 2: easy.
+            constructor; cbn.
+            exact H2. intros. now rewrite H1.
+          }
+        }
+        {
+          eapply rec.
+          unfold sub, subRelt.
+          intros. psimpl. easy.
+        }
+      }
+    }
+  }
+}
+Qed.
