Examples/ElimArray.v
@@ -1,0 +1,33 @@
+From LHL.Core Require Import
+  ProgramRules
+  LogicFacts
+  SingConds
+  Program
+  ProgramFacts
+  Traces
+  Tensor
+  Logic
+  Specs.
+
+From LHL.Util Require Import
+  TransUtil
+  Tactics
+  Util.
+
+From LHL.Examples Require Import
+  ExchangerSpec
+  RandomSpec
+  ThreadLocal.
+
+Definition E T A :=
+  RandSig |+| ESigN T (ExchSig A).
+
+Definition VE T A : Spec T (E T A) :=
+  tensorSpec randSpec (tensorNSpec T (@exchSpec T A)).
+
+Definition F A := ExchSig A.
+
+Definition VF T A : Spec T (F A) :=
+  exchSpec.
+
+Definition exch {T A} (i : Name T) (v : A) : Prog (E T A) (option A)
