Examples/RandomSpec.v
@@ -1,0 +1,66 @@
+From LHL.Core Require Import
+  Program
+  Specs
+  Logic.
+
+From LHL.Util Require Import
+  Tactics
+  TransUtil
+  Util.
+
+Variant RandSig : ESig :=
+| Random (k : nat) : RandSig nat.
+
+Definition RandState T := ActiveMap T RandSig.
+
+Variant RandStep {T} : RandState T -> ThreadEvent T RandSig -> RandState T -> Prop :=
+| CallRand i m k : RandStep
+    (fun j => if i =? j then None else m j)
+    (i, CallEv (Random k))
+    (fun j => if i =? j then Some (existT _ _ (Random k)) else m j)
+| RetRand i m k n : n <= k -> RandStep
+    (fun j => if i =? j then Some (existT _ _ (Random k)) else m j)
+    (i, RetEv (Random k) n)
+    (fun j => if i =? j then None else m j).
+
+Program Definition randSpec {T} : Spec T RandSig := {|
+  State := RandState T;
+  Step := RandStep;
+  Init _ := None
+|}.
+
+Next Obligation.
+generalize dependent (fun _ : Name T => @None {A & RandSig A}).
+intros. induction H. constructor.
+ddestruct H.
+{
+  eapply SCCall with
+    (a':=fun j =>
+      if i =? j then
+        Some (existT _ _ (Random k))
+      else
+        m j).
+  { now rewrite eqb_id. }
+  { now rewrite eqb_id. }
+  {
+    unfold differ_pointwise. intros.
+    now rewrite eqb_nid.
+  }
+  { easy. }
+}
+{
+  eapply SCRet with
+    (a':=fun j =>
+      if i =? j then
+        None
+      else
+        m j).
+  { now rewrite eqb_id. }
+  { now rewrite eqb_id. }
+  {
+    unfold differ_pointwise. intros.
+    now rewrite eqb_nid.
+  }
+  { easy. }
+}
+Qed.
