Examples/WaitFreeStackSpec.v
@@ -1,0 +1,83 @@
+From LHL.Core Require Import
+  Program
+  Specs
+  Logic.
+
+From LHL.Util Require Import
+  Tactics
+  TransUtil
+  Util.
+
+Variant StkRet {A} :=
+| PASS (v : A)
+| FAIL.
+Arguments StkRet : clear implicits.
+
+Variant WaitFreeStackSig {A} : ESig :=
+| WFPush (v : A) : WaitFreeStackSig (StkRet unit)
+| WFPop : WaitFreeStackSig (StkRet (option A)).
+Arguments WaitFreeStackSig : clear implicits.
+
+Record WaitFreeStackPend {T A} := MkWFSPend {
+  StkRetTy : Type;
+  StkName : Name T;
+  StkCall : WaitFreeStackSig A StkRetTy
+}.
+Arguments WaitFreeStackPend : clear implicits.
+Arguments MkWFSPend {T A StkRetTy}.
+
+Definition WFSPend T A:=
+  option (option (WaitFreeStackPend T A) * WaitFreeStackPend T A).
+
+Notation NoPend :=
+  (None : WFSPend _ _).
+Notation PassPend i m :=
+  (Some (None, MkWFSPend i m) : WFSPend _ _).
+Notation FailPend j mf i mp :=
+  (Some (Some (MkWFSPend j mf), MkWFSPend i mp)).
+
+Variant WaitFreeStackState {T A} :=
+| WaitFreeStackDef (vs : list A) (m : WFSPend T A).
+Arguments WaitFreeStackState : clear implicits.
+
+Variant WaitFreeStackStep {T A} : WaitFreeStackState T A -> ThreadEvent T (WaitFreeStackSig A) -> WaitFreeStackState T A -> Prop :=
+| StackCall i R (m : _ R) vs :
+    WaitFreeStackStep
+      (WaitFreeStackDef vs NoPend)
+      (i, CallEv m)
+      (WaitFreeStackDef vs (PassPend i m))
+| StackContendCall i j vs RO (mo : _ RO) RN (mn : _ RN) :
+    i <> j ->
+    WaitFreeStackStep
+      (WaitFreeStackDef vs (PassPend i mo))
+      (j, CallEv mn)
+      (WaitFreeStackDef vs (FailPend j mn i mo))
+| StackContendRet i j vs RO (mo : _ RO) RN (mn : _ (StkRet RN)) :
+    i <> j ->
+    WaitFreeStackStep
+      (WaitFreeStackDef vs (FailPend j mn i mo))
+      (j, RetEv mn FAIL)
+      (WaitFreeStackDef vs (PassPend i mo))
+| RetPush i v vs :
+    WaitFreeStackStep
+      (WaitFreeStackDef vs (PassPend i (WFPush v)))
+      (i, RetEv (WFPush v) (PASS tt))
+      (WaitFreeStackDef (v :: vs) NoPend)
+| RetPopPass i v vs :
+    WaitFreeStackStep
+      (WaitFreeStackDef (v :: vs) (PassPend i WFPop))
+      (i, RetEv WFPop (PASS (Some v)))
+      (WaitFreeStackDef vs NoPend)
+| RetPopFail i :
+    WaitFreeStackStep
+      (WaitFreeStackDef nil (PassPend i WFPop))
+      (i, RetEv WFPop (PASS None))
+      (WaitFreeStackDef nil NoPend).
+
+Program Definition wfStackSpec {T A} : Spec T (WaitFreeStackSig A) := {|
+  State := WaitFreeStackState T A;
+  Step := WaitFreeStackStep;
+  Init := WaitFreeStackDef nil NoPend
+|}.
+
+Admit Obligations.
